remembering variables

Imp/context.v
@@ -20,3 +20,62 @@ Class hasProj C X := {
 
     
 
+(* 
+
+------------------------- header.v
+
+Elpi TemplateSection 
+Section js_feature_functor. 
+
+Variables exp : Type.
+
+Variable open_rec : nat -> (e : exp) -> exp -> exp.
+
+#[induction=e, hints=[???]] (* need some way to remember when to do induction. Maybe not like this but by number?*)
+Elpi AttemptProof (open_rec).
+
+
+Elpi TemplateSection 
+End js_feature_functor. 
+
+
+------------------------- exp_lam.v
+
+#[template=js_feature_functor]
+Elpi FollowTemplateSection
+Section exp_lam.
+
+(* Defines all variables from the template *)
+
+Inductive exp_lam : Type := 
+        | ab : exp -> exp_lam
+        | app : exp -> exp -> exp_lam
+        | bvar : nat -> exp_lam
+.
+
+
+Context `{Hretr : retract exp_lam exp}.
+
+Elpi ProofObligation (Hretr).
+
+#[extends = exp] (* should it be a variable name or a "represents_as" name? Should it generate retract context decl? *)
+Elpi RegisterTypeExtension (exp_lam).
+
+(* SpecializeType open_rec exp_lam := searches for Variable open_rec, checks if it is marked with AttemptProof and replaces corresponding argument type with second argument *)
+Definition open_rec_lam : ltac:(elpi SpecializeType open_rec exp_lam). (* picks extension *)
+Proof.
+intros until e. (* from AttemptProof? *)
+elpi Induction e. (* destruct + variable calls on recursive occurrences. Maybe something like "specialized" inductive principle could be generated beforehand? Should it clear variable from context? *)
+...
+Defined. (* to be transparent *)
+
+End exp_lam.
+
+------------------------- language.v
+
+[extensions(exp_lam, exp_ite, ...)]
+Elpi Assemble signals.
+
+
+
+*)
