Imp/elpi_regestration.v
@@ -1,0 +1,418 @@
+From elpi Require Import elpi.
+
+
+
+Elpi Db section_deps.db lp:{{
+
+  % A typical Db is made of one main predicate
+  pred section_deps o:gref, o: list gref.
+
+  % the Db is empty for now, we put a rule giving a
+  % descriptive error and we name that rule "age.fail".
+  :name "section_deps.fail"
+  section_deps GRef _ :- coq.error "I don't know what" GRef "is!".
+
+  pred represents o:gref, o:string.
+
+  :name "represents.fail"
+  represents GRef _ :- coq.error "I don't know what" GRef "represents!".
+
+  pred section_deps_repr o:gref, o: list string.
+
+  :name "section_deps_repr.fail"
+  section_deps_repr GRef _ :- coq.error "I don't know what representations" GRef "depends on!".
+
+  pred represented_as o:gref, o:string.
+
+  :name "represented_as.fail"
+  represented_as GRef _ :- coq.error "I don't know what" GRef "is represented as!".
+}}.
+
+Elpi Command SetSectionDeps.
+Elpi Accumulate Db section_deps.db.
+Elpi Accumulate lp:{{
+  main [trm (global GRef)] :-
+    coq.env.transitive-dependencies GRef _ TransDep,
+    coq.env.section SectionVarsL,
+    std.filter SectionVarsL (x\ coq.gref.set.mem ( const x) TransDep) SectionVarsLRelevant,
+    std.map SectionVarsLRelevant (x\ r\ r is const x) SectionVarsLRelevantGref,
+
+    TheNewRule1 = section_deps GRef SectionVarsLRelevantGref,
+    coq.elpi.accumulate _ "section_deps.db"
+      (clause _ (before "section_deps.fail") TheNewRule1),
+
+    coq.say "Handling reprs:",
+
+    std.map SectionVarsLRelevantGref (x\ r\ (coq.say x, represents x r)) SectionVarsLRelevantRepr,
+    TheNewRule2 = section_deps_repr GRef SectionVarsLRelevantRepr,
+    coq.say "Accumulating:" TheNewRule2,
+    coq.elpi.accumulate _ "section_deps.db"
+      (clause _ (before "section_deps_repr.fail") TheNewRule2).
+}}.
+
+Elpi Command print_all_section_deps.
+Elpi Accumulate Db section_deps.db.
+Elpi Accumulate lp:{{
+
+  :before "section_deps.fail"
+  section_deps _ _ :- !, fail. % softly
+
+  :before "represents.fail"
+  represents _ _ :- !, fail. % softly
+
+  :before "section_deps_repr.fail"
+  section_deps_repr _ _ :- !, fail. % softly
+
+  :before "represented_as.fail"
+  represented_as _ _ :- !, fail. % softly
+
+  main [] :-
+    std.findall (section_deps _ _) Rules1,
+    std.findall (represents _ _) Rules2,
+    std.findall (section_deps_repr _ _) Rules3,
+    std.findall (represented_as _ _) Rules4,
+
+    std.forall Rules1 print-rule,
+    std.forall Rules2 print-rule,
+    std.forall Rules3 print-rule,
+    std.forall Rules4 print-rule.
+
+  pred print-rule i:prop.
+  print-rule (section_deps P N) :- coq.say P "depends on" N.
+  print-rule (represents P N) :- coq.say P "represents" N.
+  print-rule (section_deps_repr P N) :- coq.say P "depends on repr" N.
+  print-rule (represented_as P N) :- coq.say P "is represented as" N.
+
+}}.
+
+
+Elpi Command RegisterVariable.
+Elpi Accumulate lp:{{ 
+  pred represents o:gref, o:string.
+
+  main [str "Variable", str VName, str ":", str VTypeName] :-
+    % adding variable
+    coq.locate-all VTypeName Located,
+    std.mem Located (loc-gref TypeGR), 
+    coq.env.add-section-variable VName _ (global TypeGR) _, 
+    % looking up newly added global reference
+    coq.locate VName GRef, !, 
+    % bookkeeping
+    attributes A,
+    coq.parse-attributes A [
+      att "represents" string,
+    ] Opts,
+    (Opts =!=> (
+      (get-option "represents" ReprName; ReprName is VName),
+      TheNewRule = represents GRef ReprName,
+      coq.elpi.accumulate _ "section_deps.db" (clause _ (before "represents.fail") TheNewRule),
+      coq.say "RegVar for Any: found variable" VName "with type" TypeGR "representing" ReprName
+    )).
+
+  main [str "Variable", str VName, str ":", str "Type"] :-
+    % adding variable
+    coq.env.add-section-variable VName _ {{ Type }} _,
+    % looking up newly added global reference
+    coq.locate VName GRef,
+    % bookkeeping
+    attributes A,
+    coq.parse-attributes A [
+      att "represents" string,
+    ] Opts,
+    (Opts =!=> (
+      (get-option "represents" ReprName; ReprName is VName),
+      TheNewRule = represents GRef ReprName,
+      coq.elpi.accumulate _ "section_deps.db" (clause _ (before "represents.fail") TheNewRule), 
+      coq.say "RegVar for Type: found variable" VName "with type Type representing" ReprName
+    )).
+  main [trm (global GRef)] 
+   :- coq.say "RegVar: found gref" GRef
+    , attributes A
+    , coq.parse-attributes A [
+        att "represents" string,
+      ] Opts
+    , (Opts =!=> (
+        (get-option "represents" ReprName; ReprName is VName),
+        TheNewRule = represents GRef ReprName,
+        coq.elpi.accumulate _ "section_deps.db" (clause _ (before "represents.fail") TheNewRule), 
+        coq.say "RegVar for Type: found variable" VName "with type Type representing" ReprName
+      ))
+    .
+  main Args :- 
+    coq.say "RegVar Failure: What do" Args.
+}}.
+
+
+Section test.
+  #[represents = ARepr]
+  Elpi RegisterVariable
+  Variable A : Type.
+
+  Print A.
+
+  #[represents = xRepr]
+  Elpi RegisterVariable
+  Variable x : A.
+
+  Print x.  
+
+  
+  Variable open_rec : nat -> A -> A -> A.
+
+  #[represents = open_rec]
+  Elpi RegisterVariable (open_rec).
+
+  Elpi RegisterVariable
+  Variable y : A.
+
+  Definition id := x.
+
+  Definition id' := y.
+
+  Elpi SetSectionDeps (open_rec).
+
+  Elpi SetSectionDeps (id').  
+
+  Elpi SetSectionDeps (id).  
+
+End test.
+
+
+Elpi Command RegisterRepresented.
+Elpi Accumulate lp:{{ 
+  pred represented_as o:gref, o:string.
+
+  main [trm (global GRef)] :- 
+    attributes A,
+    coq.parse-attributes A [
+      att "represeted_as" string,
+    ] Opts,
+    (Opts =!=> (
+      (get-option "represeted_as" ReprName; ReprName is VName),
+      TheNewRule = represented_as GRef ReprName,
+      coq.elpi.accumulate _ "section_deps.db" (clause _ (before "represented_as.fail") TheNewRule), 
+      coq.say "RegisterRepresented:" GRef "is represented as" ReprName
+    )).
+
+  main Args :- 
+    coq.say "What do:" Args.
+}}.
+
+Elpi Tactic specialize_from_section.
+Elpi Accumulate Db section_deps.db.
+Elpi Accumulate lp:{{ 
+  :before "section_deps_repr.fail"
+  section_deps_repr _ _ :- !, fail. % softly
+
+  :before "represented_as.fail"
+  represented_as _ _ :- !, fail. % softly
+
+  func resolve_dependencies gref -> list (pair string (list prop)).
+  resolve_dependencies GRef DepRepMatched :- 
+    std.findall (section_deps_repr GRef _) DepReps,
+    std.mem DepReps (section_deps_repr _ DepRepList), !, 
+    coq.say "> Found gref deps:" DepRepList,
+    std.map DepRepList 
+      (x\ r\ std.findall (represented_as _ x) r
+      ) DepRepListResolved,
+    coq.say "> Resolved deps:" DepRepListResolved,
+    std.zip DepRepList DepRepListResolved DepRepMatched,
+    coq.say "> Matched deps:" DepRepMatched.
+
+  func extract (pair string (list prop)) -> gref.
+  extract P R :-
+    coq.say "Found these" P,
+    P = pr N L,
+    std.mem L (represented_as R N), !.
+
+
+  solve (goal _ _ Ty _ [str IndName] as G) GL :-
+    coq.say "Found thing:" IndName,
+    std.assert! (coq.locate IndName GRef) "can't locate",
+    coq.say "> Found gref:" GRef,
+    resolve_dependencies GRef DepRepMatched,
+    std.filter DepRepMatched (x\ x = (pr _N [])) [], !, 
+    std.map DepRepMatched extract DepRepMatched',
+    std.map DepRepMatched' (x\ r\ r is (global x)) DepRepMatched'',
+    coq.say "> Ided deps:" DepRepMatched'',
+    Res = app ((global GRef)::DepRepMatched''),
+    std.assert-ok! (coq.typecheck Res Ty) "generated term failed to typecheck",
+    coq.say Res,
+    refine Res G GL.
+
+  pred extract' i:goal-ctx i:(pair string (list prop)) o:term.
+  extract' _ P R :-
+    P = pr N L,
+    coq.say "Found these" P,
+    std.mem L (represented_as R' N), !,
+    R is (global R').
+  extract' Ctx P R :-
+    P = pr N [],
+    coq.say "Found these" P,
+    coq.string->name N N',
+    coq.say "Ctx:" Ctx,
+    % TODO: coq.name->id is for internal usage
+    std.filter Ctx (x\ x = decl _ Nn _, coq.name->id Nn N) Ctx',
+    coq.say "Ctx':" Ctx',
+    std.mem Ctx' (decl H _ Ty),
+    coq.say "found in ctx:" H  N' ":" Ty,
+    R is H.
+
+  solve (goal Ctx A TyG B [str IndName] as _G) GL :-
+    coq.say "Found thing:" IndName,
+    std.assert! (coq.locate IndName GRef) "can't locate",
+    solve (goal Ctx A TyG B [trm (global GRef)]) GL.
+
+  solve (goal Ctx _ TyG _ [trm (global GRef)] as G) GL :-
+    coq.say "> Found gref:" GRef,
+    % Resolve from databases
+    resolve_dependencies GRef DepRepMatched,
+    % Resolve from goal context
+    std.filter DepRepMatched (x\ (x = (pr N []), coq.say "Can't resolve" N)) DepRepUnresolved, !,
+    coq.say "> Unresolved deps:" DepRepUnresolved,
+    std.map DepRepMatched (x\ r\ extract' Ctx x r) DepRepMatched',
+    coq.say "> Meee deps:" DepRepMatched',
+    Res = app ((global GRef)::DepRepMatched'),
+    std.assert-ok! (coq.typecheck Res Ty) "generated term failed to typecheck",
+    coq.say "resulting term:" Res ":" Ty "while goal is" TyG,
+    refine Res G GL.
+
+  solve Args G :- 
+    coq.say "What do" Args ", G:" G,
+    coq.ltac.fail 0 "Do not know what to do".
+}}.
+
+
+Elpi Db section_template.db lp:{{
+  pred is_section_template i:string.
+
+  :name "is_section_template.fail"
+  is_section_template Name :- coq.error "I don't know this section tempalte:" Name.
+
+  pred section_vars i:string o:list (pair string string).
+
+  :name "section_vars.fail"
+  section_vars Name _ :- coq.error "I don't know this section tempalte:" Name.
+}}.
+
+
+
+Elpi Command print_all_section_vars.
+Elpi Accumulate Db section_template.db.
+Elpi Accumulate lp:{{
+
+  :before "is_section_template.fail"
+  is_section_template _ :- !, fail. % softly
+
+  :before "section_vars.fail"
+  section_vars _ _ :- !, fail. % softly
+
+  main [] :-
+    std.findall (is_section_template _) Rules1,
+    std.findall (section_vars _ _) Rules2,
+
+    std.forall Rules1 print-rule,
+    std.forall Rules2 print-rule.
+
+  pred print-rule i:prop.
+  print-rule (is_section_template P) :- coq.say "section" P.
+  print-rule (section_vars P N) :- coq.say "Variables" P N.
+
+}}.
+
+Elpi Command SectionTemplate.
+#[synterp] Elpi Accumulate lp:{{ 
+  main [str "Section", str SectionName]
+  :-  coq.say "synterop: Found section template:" SectionName
+    , coq.env.begin-section SectionName
+    .
+  main [str SectionName]
+  :-  coq.say "synterop: middle" SectionName
+    % , coq.env.end-section
+    .
+  
+  main [str "End", str SectionName]
+  :-  coq.say "synterop: Ending section template:" SectionName
+    , coq.env.end-section
+    .
+}}.
+Elpi Accumulate Db section_template.db.
+Elpi Accumulate lp:{{ 
+
+  :name "is_section_template.soft_fail"
+  :before "is_section_template.fail"
+  is_section_template _ :- !, fail. % softly
+
+  :name "section_vars.soft_fail"
+  :before "section_vars.fail"
+  section_vars _ _ :- !, fail. % softly
+  
+  main [str "Section", str SectionName]
+  :-  coq.say "Found section template:" SectionName
+    , if (is_section_template SectionName) (coq.error "Template with this name exists:" SectionName) true
+    , TheNewRule = is_section_template SectionName
+    , coq.env.begin-section SectionName
+    , coq.elpi.accumulate _ "section_template.db" (clause _ (before "is_section_template.fail") TheNewRule)
+    , coq.say "Printing:"
+    , coq.say "Added new template" SectionName
+    .
+  main [str SectionName] 
+  :-  coq.say "middle"
+    , coq.env.section Variables
+    , std.map Variables (x\ r\ coq.typecheck (global (const x)) Ty ok, std.any->string Ty r) VariableTys
+    , std.map Variables (x\ r\ r is {std.any->string x}) Variables'
+    , std.zip Variables' VariableTys R
+    , coq.say "Variables:" R
+    , TheNewRule = section_vars SectionName R
+    , coq.elpi.accumulate _ "section_template.db" (clause _ (before "section_vars.fail") TheNewRule)
+    , coq.say "Accumulated"
+    .
+  main [str "End", str SectionName]
+  :-  coq.say "Ending section template:" SectionName
+    , coq.env.current-section-path SecPath
+    , if (std.rev SecPath (SectionName::_)) true (coq.error "Trying to close mismatching section:" SectionName "Current section path:" SecPath)
+    , if (is_section_template SectionName)  true (coq.error "Trying to close section that does not exist:" SectionName) 
+    , coq.env.end-section
+    .
+  main Args 
+  :-  coq.say "What do: " Args
+    .
+}}.
+
+Elpi Command What.
+Elpi Accumulate lp:{{ 
+pred section_vars i:string o:list (pair string string).
+
+main [str SectionName] 
+  :- coq.say "middle"
+   , coq.env.section Variables
+   , std.map Variables (x\ r\ coq.typecheck (global (const x)) Ty ok, std.any->string Ty r) VariableTys
+   , std.map Variables (x\ r\ r is {std.any->string x}) Variables'
+   , std.zip Variables' VariableTys R
+   , coq.say "Variables:" R
+   , TheNewRule = section_vars SectionName R
+   , coq.elpi.accumulate _ "section_template.db" (clause _ (before "section_vars.fail") TheNewRule)
+   , coq.say "Accumulated"
+  .
+}}.
+
+Elpi SectionTemplate
+Section exp_lam'.
+
+    Variable exp : Type.
+    
+    Inductive exp_lam : Type := 
+        | ab : exp -> exp_lam
+        | app : exp -> exp -> exp_lam
+        | bvar : nat -> exp_lam
+    .
+
+Elpi What "exp_lam'".
+
+Elpi print_all_section_vars.
+
+Elpi SectionTemplate
+End exp_lam'.
+
+(* End exp_lam'. *)
+
