Imp/elpi_section_template.v
@@ -1,0 +1,102 @@
+From elpi Require Import elpi.
+
+Elpi Db section_template.db lp:{{
+
+  pred is_section_template o:string.
+  pred section_template_vars o:string o:list (pair string term).
+
+  % the Db is empty for now, we put a rule giving a
+  % descriptive error and we name that rule "age.fail".
+  :name "is_section_template.fail"
+  is_section_template Name :- coq.error "I don't know who" Name "is!".
+
+  :name "section_template_vars.fail"
+  section_template_vars Name _ :- coq.error "I don't know this section tempalte:" Name.
+
+}}.
+
+
+Elpi Command print_all_section_template.
+Elpi Accumulate Db section_template.db.
+Elpi Accumulate lp:{{
+
+  :before "is_section_template.fail"
+  is_section_template _ :- !, fail. % softly
+
+  main [] :-
+    std.findall (is_section_template _) Rules,
+    std.forall Rules print-rule.
+
+  pred print-rule i:prop.
+  print-rule (is_section_template P) :- coq.say "found" P .
+
+}}.
+
+Elpi Command print_all_section_template_vars.
+Elpi Accumulate lp:{{
+
+  :before "section_template_vars.fail"
+  section_template_vars _ _ :- !, fail. % softly
+
+  main [] :-
+    std.findall (section_template_vars _ _) Rules,
+    std.forall Rules print-rule.
+
+  pred print-rule i:prop.
+  print-rule (section_template_vars P N) :- coq.say "Section" P "has these vars" N.
+
+}}.
+
+Elpi Command SectionTemplate.
+#[synterp] Elpi Accumulate lp:{{ 
+  main [str "Section", str SectionName]
+  :-  coq.say "synterop: Found section template:" SectionName
+    , coq.env.begin-section SectionName
+    .
+  main [str SectionName]
+  :-  coq.say "synterop: middle" SectionName
+    % , coq.env.end-section
+    .
+  
+  main [str "End", str SectionName]
+  :-  coq.say "synterop: Ending section template:" SectionName
+    , coq.env.end-section
+    .
+}}.
+Elpi Accumulate Db is_section_template.db.
+Elpi Accumulate Db section_template_vars.db.
+Elpi Accumulate lp:{{ 
+
+  :before "is_section_template.fail"
+  is_section_template _ :- !, fail. % softly
+
+  :before "section_template_vars.fail"
+  section_template_vars _ _ :- !, fail. % softly
+  
+  main [str "Section", str SectionName]
+  :-  coq.say "Found section template:" SectionName
+    , if (is_section_template SectionName) (coq.error "Template with this name exists:" SectionName) true
+    , TheNewRule = is_section_template SectionName
+    , coq.env.begin-section SectionName
+    , coq.elpi.accumulate _ "is_section_template.db" (clause _ (before "is_section_template.fail") TheNewRule)
+    , coq.say "Printing:"
+    , coq.say "Added new template" SectionName
+    .
+  main [str "End", str SectionName]
+  :-  coq.say "Ending section template:" SectionName
+    , coq.env.section Variables
+    , std.map Variables (x\ r\ coq.typecheck (global (const x)) r ok) VariableTys
+    , std.map Variables (x\ r\ r is {std.any->string x}) Variables'
+    , std.zip Variables' VariableTys R
+    , coq.say "Variables:" R
+    , TheNewRule = section_template_vars SectionName R
+    , coq.elpi.accumulate _ "section_template_vars.db" (clause _ (before "section_template_vars.fail") TheNewRule)
+    , coq.env.current-section-path SecPath
+    , if (std.rev SecPath (SectionName::_)) true (coq.error "Trying to close mismatching section:" SectionName "Current section path:" SecPath)
+    , if (is_section_template SectionName)  true (coq.error "Trying to close section that does not exist:" SectionName) 
+    , coq.env.end-section
+    .
+  main Args 
+  :-  coq.say "What do: " Args
+    .
+}}.
