Imp/signals.v
@@ -8,10 +8,55 @@ From Imp Require Import int_lam_err int_ite_err int_mut_err.
 
 From elpi Require Import elpi.
 
-(*  *)
+Elpi Export specialize_from_section.  
 
-Elpi Export specialize_from_section.
 
+(*
+TODO:
+1. Generate specialized versions of non-recursive terms.
+2. Make tactic for generating specialized recursive terms in their closing definitions
+    a. Mark one argument as "structurally" decreasing and supply it after induction?
+3. Template section? It seems that variables in sections and language properties mirror each other. 
+   It might be beneficial to have a common source of truth for both of them.
+
+   Maybe it should be a map from names to types that is discharged to sections for proofs 
+
+   Elpi TemplateSection feature_functor.
+        Variable exp : Type.
+        Context `{Hretr : retract ?exp_lam exp}.
+
+        Elpi MarkInduction 1 (* ----v *)
+        Variable open_rec : nat -> exp -> exp -> exp. 
+        ...
+        ...
+        ...
+        Variable preservation : forall c e c' e', lc' 0 e -> step c e c' e' -> lc' 0 e'.
+
+
+   Elpi End feature_functor.
+
+   #[template=feature_functor]
+   Elpi FollowTemplate
+   Section exp_lam.
+     (* all variables from feature_functor are defined and registered *)
+
+   End exp_lam.
+
+   #[template=feature_functor]
+   Elpi RealizeTemplate.
+
+   Should generate proof obligations for each variable and try to prove them by induction and auto?
+   Maybe it should be a record? 
+   
+*)
+
+
+(* 
+
+Inductive exp = Elpi Fix (exp_ite |+| exp_mut |+| exp_err |+| exp_lam).
+
+
+*)
 
 Inductive exp : Type := 
     | In_exp_lam : (specialize_from_section exp_lam) -> exp
@@ -20,6 +65,9 @@ Inductive exp : Type :=
     | In_exp_err : exp_err exp -> exp
 .
 
+(* Probably is a good idea to do 
+    1. typechecking for corresponding mark
+    2. give warning if no such mark exists *)
 #[represeted_as = exp]
 Elpi RegisterRepresented (exp).
 
@@ -68,6 +116,8 @@ end.
 #[represeted_as = retract_exp_exp_lam]
 Elpi RegisterRepresented (retract_exp_exp_lam).
 
+Check open_rec_lam.
+
 Fixpoint open_rec (k : nat) (u : exp) (e : exp) : exp := 
     match e with 
         (* | In_exp_lam e => open_rec_lam _ open_rec k u e *)
@@ -78,12 +128,12 @@ Fixpoint open_rec (k : nat) (u : exp) (e : exp) : exp :=
     end
 .
 
-
-
 #[represeted_as = open_rec]
 Elpi RegisterRepresented (open_rec).
 
-Definition open_rec_lam' := ltac:(elpi specialize_from_section open_rec_lam).
+Definition open_rec_lam' :=  ltac:(elpi specialize_from_section open_rec_lam).
+
+Check open_rec_lam'.
 
 Inductive lc' : nat -> exp -> Prop := 
     | lc_in_lam n e : lc'_lam _ lc' n e -> lc' n e
@@ -116,15 +166,24 @@ Definition retract_open_rec_rev exp_ext open_rec_ext  { retr : retract_f exp_ext
     forall (n : nat) s (e : exp_ext exp), open_rec n s (inj e) = open_rec_ext retr open_rec n s e.
 
 
-Definition retract_open_rec_rev_lam : 
-    forall (n : nat) s (e : exp_lam exp), open_rec n s (inj e) = open_rec_lam' n s e := ltac:(intros; easy).
+Definition retract_open_rec_rev_lam : forall (n : nat) s (e : exp_lam exp)
+                                    , open_rec n s (inj e) = open_rec_lam exp open_rec n s e 
+                                    := ltac:(intros; easy).
+
+Definition retract_open_rec_rev_ite : forall (n : nat) s (e : exp_ite exp)
+                                    , open_rec n s (inj e) = open_rec_ite exp open_rec n s e 
+                                    := ltac:(intros; easy).
+
+Definition retract_open_rec_rev_mut : forall (n : nat) s (e : exp_mut exp)
+                                    , open_rec n s (inj e) = open_rec_mut exp open_rec n s e 
+                                    := ltac:(intros; easy).
+
+Definition retract_open_rec_rev_err : forall (n : nat) s (e : exp_err exp)
+                                    , open_rec n s (inj e) = open_rec_err exp open_rec n s e 
+                                    := ltac:(intros; easy).
 
 #[represeted_as = retract_open_rec_rev_lam]
 Elpi RegisterRepresented (retract_open_rec_rev_lam).
-
-Definition retract_open_rec_rev_ite : retract_open_rec_rev exp_ite (@open_rec_ite exp) := ltac:(intros; easy).
-Definition retract_open_rec_rev_mut : retract_open_rec_rev exp_mut (@open_rec_mut exp) := ltac:(intros; easy).
-Definition retract_open_rec_rev_err : retract_open_rec_rev exp_err (@open_rec_err exp) := ltac:(intros; easy).
 
 Fixpoint lc_weaken   : forall s n m, n <= m -> lc' n s -> lc' m s.
 inversion 2; subst.
@@ -274,7 +333,8 @@ Defined.
 Elpi RegisterRepresented (ctx_supports_store).
 
 Inductive step : Ctx -> exp -> Ctx -> exp -> Prop := 
-    | step_in_lam (c : Ctx) s c' s' : step_lam _ open_rec value _ step c s c' s' -> step c s c' s'
+    (* | step_in_lam (c : Ctx) s c' s' : step_lam _ open_rec value _ step c s c' s' -> step c s c' s' *)
+    | step_in_lam (c : Ctx) s c' s' : (specialize_from_section step_lam) c s c' s' -> step c s c' s'
     | step_in_ite (c : Ctx) s c' s' : step_ite _ _                step c s c' s' -> step c s c' s'
     | step_in_mut (c : Ctx) s c' s' : step_mut _ _ _              step c s c' s' -> step c s c' s'
     | step_in_err (c : Ctx) s c' s' : step_err _ _                step c s c' s' -> step c s c' s'
@@ -290,11 +350,12 @@ Elpi RegisterRepresented (step).
 Definition lc := lc' 0.
 Definition open := open_rec 0.
 
-Fixpoint preservation : forall c e c' e', 
-    lc e -> 
+Fixpoint preservation : forall c e c' e',
+    lc e ->
     step c e c' e' -> 
     lc e'. 
 Proof. 
+    (* intros *. *)
     intros c e c' e'.
     unfold lc in *.
     induction 2.
@@ -312,3 +373,4 @@ Defined.
 #[represeted_as = preservation]
 Elpi RegisterRepresented (preservation).
 
+(* Fixpoint thing : forall c e c1' c2' e1' e2', lc e -> step c e c1' e1' -> step c e c2' e2' -> (c1' = c2' /\ e1' = e2'). *)
